ZKLib/OracleReduction/Composition.lean
@@ -4,7 +4,7 @@ Released under Apache 2.0 license as described in the file LICENSE.
 Authors: Quang Dao
 -/
 
-import ZKLib.OracleReduction.Security
+import ZKLib.OracleReduction.Basic
 
 /-!
   # Composition of Interactive (Oracle) Protocols with Compatible Relations
@@ -14,185 +14,275 @@ import ZKLib.OracleReduction.Security
   R3. This gives us an interactive (oracle) protocol for reducing relations R1 => R3.
 -/
 
+namespace ProtocolSpec
+
 section Restrict
 
 variable {n : ℕ}
 
-abbrev ProtocolSpec.take (m : ℕ) (h : m ≤ n) (pSpec : ProtocolSpec n) :=
-  Fin.take m h pSpec
+abbrev take (m : ℕ) (h : m ≤ n) (pSpec : ProtocolSpec n) := Fin.take m h pSpec
 
-abbrev ProtocolSpec.rtake (m : ℕ) (h : m ≤ n) (pSpec : ProtocolSpec n) :=
-  Fin.rtake m h pSpec
+abbrev rtake (m : ℕ) (h : m ≤ n) (pSpec : ProtocolSpec n) := Fin.rtake m h pSpec
 
-abbrev Transcript.take {pSpec : ProtocolSpec n} (m : ℕ) (h : m ≤ n)
-    (transcript : Transcript pSpec) : Transcript (pSpec.take m h) :=
+abbrev FullTranscript.take {pSpec : ProtocolSpec n} (m : ℕ) (h : m ≤ n)
+    (transcript : FullTranscript pSpec) : FullTranscript (pSpec.take m h) :=
   Fin.take m h transcript
 
-abbrev Transcript.rtake {pSpec : ProtocolSpec n} (m : ℕ) (h : m ≤ n)
-    (transcript : Transcript pSpec) : Transcript (pSpec.rtake m h) :=
+abbrev FullTranscript.rtake {pSpec : ProtocolSpec n} (m : ℕ) (h : m ≤ n)
+    (transcript : FullTranscript pSpec) : FullTranscript (pSpec.rtake m h) :=
   Fin.rtake m h transcript
 
 end Restrict
 
-section Composition
-
-variable {n m : ℕ}
+variable {m n : ℕ}
 
 /-- Adding a round with direction `dir` and type `Message` to the beginning of a `ProtocolSpec` -/
-abbrev ProtocolSpec.cons (pSpec : ProtocolSpec n) (dir : Direction) (Message : Type) :
-    ProtocolSpec (n + 1) :=
-  Fin.cons ⟨dir, Message⟩ pSpec
+abbrev cons (pSpec : ProtocolSpec n) (dir : Direction) (Message : Type) :
+    ProtocolSpec (n + 1) := Fin.cons ⟨dir, Message⟩ pSpec
 
 /-- Adding a round with direction `dir` and type `Message` to the end of a `ProtocolSpec` -/
-abbrev ProtocolSpec.snoc (pSpec : ProtocolSpec n) (dir : Direction) (Message : Type) :
-    ProtocolSpec (n + 1) :=
-  Fin.snoc pSpec ⟨dir, Message⟩
+abbrev snoc (pSpec : ProtocolSpec n) (dir : Direction) (Message : Type) :
+    ProtocolSpec (n + 1) := Fin.snoc pSpec ⟨dir, Message⟩
 
 /-- Appending two `ProtocolSpec`s -/
-abbrev ProtocolSpec.append (pSpec : ProtocolSpec n) (pSpec' : ProtocolSpec m) :
-    ProtocolSpec (n + m) :=
+abbrev append (pSpec : ProtocolSpec m) (pSpec' : ProtocolSpec n) : ProtocolSpec (m + n) :=
   Fin.append pSpec pSpec'
 
-def ProtocolSpec.mkSingle (dir : Direction) (Message : Type) : ProtocolSpec 1 :=
-  fun _ => ⟨dir, Message⟩
+@[inline, reducible]
+def mkSingle (dir : Direction) (Message : Type) : ProtocolSpec 1 := fun _ => ⟨dir, Message⟩
 
 infixl : 65 " ++ₚ " => ProtocolSpec.append
 
 @[simp]
-theorem ProtocolSpec.snoc_take {pSpec : ProtocolSpec n} (m : ℕ) (h : m < n) :
-    (pSpec.take m (by omega) ++ₚ (fun (_ : Fin 1) => pSpec ⟨m, h⟩))
-        = pSpec.take (m + 1) (by omega) := by
+theorem snoc_take {pSpec : ProtocolSpec n} (k : ℕ) (h : k < n) :
+    (pSpec.take k (by omega) ++ₚ (fun (_ : Fin 1) => pSpec ⟨k, h⟩))
+      = pSpec.take (k + 1) (by omega) := by
   simp only [append, take, Fin.append_right_eq_snoc, Fin.take_succ_eq_snoc]
 
-/-- Appending two `ToOracle`s for two `ProtocolSpec`s -/
-def ToOracle.append {pSpec₁ : ProtocolSpec n} {pSpec₂ : ProtocolSpec m}
-    [O₁ : ∀ i, ToOracle (pSpec₁.Message i)] [O₂ : ∀ i, ToOracle (pSpec₂.Message i)] :
-        ∀ i, ToOracle ((pSpec₁ ++ₚ pSpec₂).Message i) := fun ⟨i, h⟩ => by
-  dsimp [ProtocolSpec.append, ProtocolSpec.getDir] at h ⊢
-  by_cases h' : i < n
-  · rw [← Fin.castAdd_castLT m i h', Fin.append_left] at h ⊢
-    exact O₁ ⟨i.castLT h', h⟩
-  · rw [← @Fin.natAdd_subNat_cast n m i (not_lt.mp h'), Fin.append_right] at h ⊢
-    exact O₂ ⟨Fin.subNat n (Fin.cast (add_comm n m) i) (not_lt.mp h'), h⟩
-
-instance {pSpec : ProtocolSpec n} {pSpec' : ProtocolSpec m}
-    [∀ i, ToOracle (pSpec.Message i)] [∀ i, ToOracle (pSpec'.Message i)] :
-    ∀ i, ToOracle ((pSpec ++ₚ pSpec').Message i) := ToOracle.append
-
 /-- Appending two transcripts for two `ProtocolSpec`s -/
-def Transcript.append {pSpec₁ : ProtocolSpec n} {pSpec₂ : ProtocolSpec m}
-    (T₁ : Transcript pSpec₁) (T₂ : Transcript pSpec₂) : Transcript (pSpec₁ ++ₚ pSpec₂) := by
-  dsimp [ProtocolSpec.append, ProtocolSpec.getDir]
-  dsimp [Transcript, ProtocolSpec.getType] at T₁ T₂ ⊢
-  exact fun i => (Fin.append_comp Prod.snd i) ▸ (Fin.addCases' T₁ T₂ i)
+def FullTranscript.append {pSpec₁ : ProtocolSpec m} {pSpec₂ : ProtocolSpec n}
+    (T₁ : FullTranscript pSpec₁) (T₂ : FullTranscript pSpec₂) :
+        FullTranscript (pSpec₁ ++ₚ pSpec₂) := by
+  dsimp only [ProtocolSpec.append, ProtocolSpec.getDir, FullTranscript, ProtocolSpec.getType]
+    at T₁ T₂ ⊢
+  exact fun i => (Fin.append_comp' Prod.snd i) ▸ (Fin.addCases' T₁ T₂ i)
 
-infixl : 65 " ++ₜ " => Transcript.append
+infixl : 65 " ++ₜ " => FullTranscript.append
 
 /-- Adding a message with a given direction and type to the end of a `Transcript` -/
-def Transcript.snoc {pSpec : ProtocolSpec n} {NextMessage : Type}
-    (T : Transcript pSpec) (dir : Direction) (msg : NextMessage) :
-        Transcript (pSpec ++ₚ .mkSingle dir NextMessage) :=
-  Transcript.append T fun _ => msg
+def FullTranscript.snoc {pSpec : ProtocolSpec n} {NextMessage : Type}
+    (T : FullTranscript pSpec) (dir : Direction) (msg : NextMessage) :
+        FullTranscript (pSpec ++ₚ .mkSingle dir NextMessage) :=
+  FullTranscript.append T fun _ => msg
 
-end Composition
+section Test
 
-section Composition
+def pSpecTest : ProtocolSpec 2 := ![⟨.P_to_V, Nat⟩, ⟨.V_to_P, Rat⟩]
 
-variable {n m : ℕ} {pSpec₁ : ProtocolSpec n} {pSpec₂ : ProtocolSpec m} {ι : Type} [DecidableEq ι]
-    {oSpec : OracleSpec ι} {Stmt₁ Wit₁ Stmt₂ Wit₂ Stmt₃ Wit₃ PrvState : Type}
+def pSpecCombined : ProtocolSpec 4 := pSpecTest ++ₚ pSpecTest
+
+theorem pSpecCombined_eq :
+    pSpecCombined = ![⟨.P_to_V, Nat⟩, ⟨.V_to_P, Rat⟩, ⟨.P_to_V, Nat⟩, ⟨.V_to_P, Rat⟩] := by
+  funext i
+  dsimp only [pSpecCombined, pSpecTest, ProtocolSpec.append, Fin.append, Fin.addCases, Fin.castLT,
+    Fin.subNat, Fin.cast]
+  fin_cases i <;> simp
+
+end Test
+
+variable {pSpec₁ : ProtocolSpec m} {pSpec₂ : ProtocolSpec n}
 
 @[simp]
-theorem ProtocolSpec.take_append_left :
-    (pSpec₁ ++ₚ pSpec₂).take n (Nat.le_add_right n m) = pSpec₁ := by
+theorem take_append_left :
+    (pSpec₁ ++ₚ pSpec₂).take m (Nat.le_add_right m n) = pSpec₁ := by
   simp only [take, append]
-  have {i : Fin n} : Fin.castLE (by omega) i = Fin.castAdd m i := by
+  have {i : Fin m} : Fin.castLE (by omega) i = Fin.castAdd n i := by
     simp only [Fin.castLE, Fin.castAdd]
   ext i <;>
   simp only [Fin.take_apply, this, Fin.append_left]
 
 @[simp]
-theorem Transcript.take_append_left (T : Transcript pSpec₁) (T' : Transcript pSpec₂) :
-    ((T ++ₜ T').take n (Nat.le_add_right n m)) =
-      (@ProtocolSpec.take_append_left _ _ pSpec₁ pSpec₂).symm ▸ T := by
-  simp [Transcript.append, Transcript.take]
+theorem Transcript.take_append_left (T : FullTranscript pSpec₁) (T' : FullTranscript pSpec₂) :
+    ((T ++ₜ T').take m (Nat.le_add_right m n)) =
+      (@take_append_left _ _ pSpec₁ pSpec₂).symm ▸ T := by
+  simp [FullTranscript.append, FullTranscript.take, ProtocolSpec.append]
   ext i
   simp [Fin.castLE, Fin.addCases', Fin.addCases, eqRec_eq_cast, cast_eq_iff_heq]
+  refine heq_of_eq_cast ?_ ?_
+  simp [Fin.append, Fin.addCases]
+  simp [cast]
   sorry
 
--- def ProverRound.append (P : ProverRound pSpec₁ oSpec PrvState)
---     (P' : ProverRound pSpec₂ oSpec PrvState) :
---     ProverRound (pSpec₁ ++ₚ pSpec₂) oSpec PrvState := sorry
-  -- receiveChallenge := fun ⟨i, h⟩ => by
-  --   refine Fin.addCases ?_ ?_ i <;> intro j c <;>
-  --   simp [ProtocolSpec.append] at c ⊢
-  --   · exact P.receiveChallenge j c
-  --   · exact P'.receiveChallenge j c
-  -- sendMessage := fun ⟨i, h⟩ => by
-  --   refine Fin.addCases ?_ ?_ i <;> intro j c <;>
-  --   simp [ProtocolSpec.append] at c ⊢
-  --   · exact P.sendMessage j c
-  --   · exact P'.sendMessage j c
+theorem Transcript.eq_left_of_append (k : Fin (m + 1))
+    (T : Transcript ⟨k, by omega⟩ (pSpec₁ ++ₚ pSpec₂)) : True := sorry
+  --   (T.take m (by omega)).cast (by simp) = T.cast (by simp) := by
+  -- sorry
 
-def Prover.append (P : Prover pSpec₁ oSpec Stmt₁ Wit₁ Stmt₂ Wit₂)
-    (P' : Prover pSpec₂ oSpec Stmt₂ Wit₂ Stmt₃ Wit₃) :
-        Prover (pSpec₁ ++ₚ pSpec₂) oSpec Stmt₁ Wit₁ Stmt₃ Wit₃ where
-  PrvState := Fin.append (m := n) (Fin.init P.PrvState) P'.PrvState
-  load := sorry
-  sendMessage := sorry
-  receiveChallenge := sorry
-  output := sorry
+def FullTranscript.fst (T : FullTranscript (pSpec₁ ++ₚ pSpec₂)) : FullTranscript pSpec₁ :=
+  fun i => by
+    simpa only [getType_apply, ProtocolSpec.append, Fin.append_left] using T (Fin.castAdd n i)
+
+def FullTranscript.snd (T : FullTranscript (pSpec₁ ++ₚ pSpec₂)) : FullTranscript pSpec₂ :=
+  fun i => by
+    simpa only [getType_apply, ProtocolSpec.append, Fin.append_right] using T (Fin.natAdd m i)
+
+end ProtocolSpec
+
+open ProtocolSpec
+
+variable {m n : ℕ} {pSpec₁ : ProtocolSpec m} {pSpec₂ : ProtocolSpec n} {ι : Type} [DecidableEq ι]
+    {oSpec : OracleSpec ι} {Stmt₁ Wit₁ Stmt₂ Wit₂ Stmt₃ Wit₃ : Type}
+
+/-- Appending two `ToOracle`s for two `ProtocolSpec`s -/
+def ToOracle.append [O₁ : ∀ i, ToOracle (pSpec₁.Message i)]
+    [O₂ : ∀ i, ToOracle (pSpec₂.Message i)] :
+      ∀ i, ToOracle ((pSpec₁ ++ₚ pSpec₂).Message i) := fun ⟨i, h⟩ => by
+  dsimp [ProtocolSpec.append, ProtocolSpec.getDir] at h ⊢
+  by_cases h' : i < m
+  · rw [← Fin.castAdd_castLT n i h', Fin.append_left] at h ⊢
+    exact O₁ ⟨i.castLT h', h⟩
+  · rw [← @Fin.natAdd_subNat_cast m n i (not_lt.mp h'), Fin.append_right] at h ⊢
+    exact O₂ ⟨Fin.subNat m (Fin.cast (add_comm m n) i) (not_lt.mp h'), h⟩
+
+instance [∀ i, ToOracle (pSpec₁.Message i)] [∀ i, ToOracle (pSpec₂.Message i)] :
+    ∀ i, ToOracle ((pSpec₁ ++ₚ pSpec₂).Message i) := ToOracle.append
+
+#print ToOracle.append
+
+/--
+Appending two provers corresponding to two reductions, where the output statement & witness type for
+the first prover is equal to the input statement & witness type for the second prover. We also
+require a verifier for the first protocol in order to derive the intermediate statement for the
+second prover.
+
+This is defined by combining the two provers' private states and functions, with the exception that
+the last private state of the first prover is "merged" into the first private state of the second
+prover (via outputting the new statement and witness, and then inputting these into the second
+prover). -/
+def Prover.append (P₁ : Prover pSpec₁ oSpec Stmt₁ Wit₁ Stmt₂ Wit₂)
+    (P₂ : Prover pSpec₂ oSpec Stmt₂ Wit₂ Stmt₃ Wit₃) :
+      Prover (pSpec₁ ++ₚ pSpec₂) oSpec Stmt₁ Wit₁ Stmt₃ Wit₃ where
+
+  /- The combined prover's states are the concatenation of the first prover's states, except the
+  last one, and the second prover's states. -/
+  PrvState := Fin.append (m := m) (Fin.init P₁.PrvState) P₂.PrvState ∘ Fin.cast (by omega)
+
+  /- The combined prover's input function is the first prover's input function, except for when the
+  first protocol is empty, in which case it is the second prover's input function -/
+  input := fun stmt wit => by
+    by_cases h : m > 0
+    · simp [Fin.append, Fin.addCases, Fin.init, Fin.castLT, h]
+      exact P₁.input stmt wit
+    · simp [Fin.append, Fin.addCases, h, Fin.subNat]
+      exact (do
+        let state ← P₁.input stmt wit
+        haveI : 0 = Fin.last m := by aesop
+        haveI state : P₁.PrvState (Fin.last m) := by simpa [this] using state
+        return ← P₂.input.uncurry (P₁.output state))
+
+  /- The combined prover sends messages according to the round index `i` as follows:
+  - if `i < m - 1`, then it sends the message & updates the state as the first prover
+  - if `i = m - 1`, then it sends the message as the first prover, but further returns the beginning
+    state of the second prover
+  - if `i > m`, then it sends the message & updates the state as the second prover. It needs to
+    provide a `stmt₂` for the second prover, which it derives from running the verifier on the first
+    transcript. -/
+  sendMessage := fun ⟨⟨i, hLt⟩, h⟩ state => by
+    by_cases hi : i < m
+    · simp [ProtocolSpec.append, Fin.append, Fin.addCases, Fin.init, hi,
+        Fin.cast, Fin.castLT, Fin.succ, Fin.castSucc] at h state ⊢
+      by_cases hi' : i + 1 < m
+      · simp [hi']
+        exact P₁.sendMessage ⟨⟨i, hi⟩, h⟩ state
+      · haveI : i + 1 = m := by omega
+        simp [this]
+        exact (do
+          let ⟨msg, state⟩ ← P₁.sendMessage ⟨⟨i, hi⟩, h⟩ state
+          haveI state : P₁.PrvState (Fin.last m) := by
+            simpa [Fin.last, this] using state
+          return ⟨msg, ← P₂.input.uncurry (P₁.output state)⟩)
+    · haveI : ¬ i + 1 < m := by omega
+      simp [ProtocolSpec.append, Fin.append, Fin.addCases, Fin.init, hi, this,
+        Fin.cast, Fin.castLT, Fin.succ, Fin.castSucc] at h state ⊢
+      exact (do
+        let ⟨msg, newState⟩ ← P₂.sendMessage ⟨⟨i - m, by omega⟩, h⟩ state
+        haveI newState : P₂.PrvState ⟨i + 1 - m, by omega⟩ := by
+          haveI : i + 1 - m = i - m + 1 := by omega
+          simpa [Fin.succ, this] using newState
+        return ⟨msg, newState⟩)
+
+  /- Receiving challenges is implemented essentially the same as sending messages, modulo the
+  difference in direction. -/
+  receiveChallenge := fun ⟨⟨i, hLt⟩, h⟩ state chal => by
+    by_cases hi : i < m
+    · simp [ProtocolSpec.append, Fin.append, Fin.addCases, Fin.init, hi,
+        Fin.cast, Fin.castLT, Fin.succ, Fin.castSucc] at h state chal ⊢
+      by_cases hi' : i + 1 < m
+      · simp [hi']
+        exact P₁.receiveChallenge ⟨⟨i, hi⟩, h⟩ state chal
+      · haveI : i + 1 = m := by omega
+        simp [this]
+        exact (do
+          let newState ← P₁.receiveChallenge ⟨⟨i, hi⟩, h⟩ state chal
+          haveI newState : P₁.PrvState (Fin.last m) := by
+            simpa [Fin.last, this] using newState
+          return ← P₂.input.uncurry (P₁.output newState))
+    · haveI : ¬ i + 1 < m := by omega
+      simp [ProtocolSpec.append, Fin.append, Fin.addCases, Fin.init, hi, this,
+        Fin.cast, Fin.castLT, Fin.succ, Fin.castSucc] at h state chal ⊢
+      exact (do
+        let newState ← P₂.receiveChallenge ⟨⟨i - m, by omega⟩, h⟩ state chal
+        haveI newState : P₂.PrvState ⟨i + 1 - m, by omega⟩ := by
+          haveI : i + 1 - m = i - m + 1 := by omega
+          simpa [Fin.succ, this] using newState
+        return newState)
+
+  /- The combined prover's output function is simply the second prover's output function. -/
+  output := fun state => by
+    simp [Fin.append, Fin.addCases, Fin.last] at state
+    exact P₂.output state
 
 /-- Composition of verifiers. Return the conjunction of the decisions of the two verifiers. -/
-def Verifier.append (V : Verifier pSpec₁ oSpec Stmt₁ Stmt₂)
-    (V' : Verifier pSpec₂ oSpec Stmt₂ Stmt₃) :
-        Verifier (pSpec₁ ++ₚ pSpec₂) oSpec Stmt₁ Stmt₃ := sorry
-  -- verify := fun stmt transcript => do
-  --   let firstTranscript : Transcript pSpec₁ := by
-  --     have := transcript.take n (by omega)
-  --     simp at this; exact this
-  --   let decision ← V.verify stmt firstTranscript
-    -- let secondTranscript : Transcript pSpec₂ := by
+def Verifier.append (V₁ : Verifier pSpec₁ oSpec Stmt₁ Stmt₂)
+    (V₂ : Verifier pSpec₂ oSpec Stmt₂ Stmt₃) :
+      Verifier (pSpec₁ ++ₚ pSpec₂) oSpec Stmt₁ Stmt₃ where
+  verify := fun stmt transcript => do
+    return ← V₂.verify (← V₁.verify stmt transcript.fst) transcript.snd
+
+/-- Composition of reductions boils down to composing the provers and verifiers. -/
+def Reduction.append (R₁ : Reduction pSpec₁ oSpec Stmt₁ Wit₁ Stmt₂ Wit₂)
+    (R₂ : Reduction pSpec₂ oSpec Stmt₂ Wit₂ Stmt₃ Wit₃) :
+      Reduction (pSpec₁ ++ₚ pSpec₂) oSpec Stmt₁ Wit₁ Stmt₃ Wit₃ where
+  prover := Prover.append R₁.prover R₂.prover
+  verifier := Verifier.append R₁.verifier R₂.verifier
+
+variable [O₁ : ∀ i, ToOracle (pSpec₁.Message i)] [O₂ : ∀ i, ToOracle (pSpec₂.Message i)]
+
+def OracleVerifier.append (V : OracleVerifier pSpec₁ oSpec Stmt₁ Stmt₂)
+    (V' : OracleVerifier pSpec₂ oSpec Stmt₂ Stmt₃) :
+      OracleVerifier (pSpec₁ ++ₚ pSpec₂) oSpec Stmt₁ Stmt₃ where
+  genQueries := fun stmt transcript => do sorry
+    -- let queries ← V.genQueries stmt transcript.fst.challenges
+    -- let queries' ← V'.genQueries stmt transcript.snd.challenges
+    -- return queries ++ queries'
+  verify := fun stmt transcript responseList => do sorry
+    -- let firstTranscript : FullTranscript pSpec₁ := by
+    --   have := transcript.take n (by omega)
+    --   simp at this; exact this
+    -- let stmt₂ ← V.verify stmt firstTranscript
+    -- let secondTranscript : FullTranscript pSpec₂ := by
     --   have := transcript.rtake m (by omega)
     --   sorry
-    -- let decision' ← V'.verify stmt secondTranscript
-    -- return decision ∧ decision'
+    -- return ← V'.verify stmt₂ secondTranscript
 
-def Reduction.append (P : Reduction pSpec₁ oSpec Stmt₁ Wit₁ Stmt₂ Wit₂)
-    (P' : Reduction pSpec₂ oSpec Stmt₂ Wit₂ Stmt₃ Wit₃) :
-    Reduction (pSpec₁ ++ₚ pSpec₂) oSpec Stmt₁ Wit₁ Stmt₃ Wit₃ := sorry
-  -- prover := Prover.append P.prover P'.prover
-  -- verifier := Verifier.append P.verifier P'.verifier
-
-def OracleVerifier.append [O : ∀ i, ToOracle (pSpec₁.Message i)]
-    [O' : ∀ i, ToOracle (pSpec₂.Message i)] (V : OracleVerifier pSpec₁ oSpec Stmt₁ Stmt₂)
-    (V' : OracleVerifier pSpec₂ oSpec Stmt₂ Stmt₃) :
-        OracleVerifier (pSpec₁ ++ₚ pSpec₂) oSpec Stmt₁ Stmt₃ := sorry
-  -- genQueries := fun stmt transcript => do
-  --   let queries ← V.genQueries stmt transcript.challenges
-  --   let queries' ← V'.genQueries stmt transcript.challenges
-  --   return queries ++ queries'
-  -- verify := fun stmt transcript responseList => do
-  --   let firstTranscript : Transcript pSpec₁ := by
-  --     have := transcript.take n (by omega)
-  --     simp at this; exact this
-  --   let decision ← V.verify stmt firstTranscript
-  --   let secondTranscript : Transcript pSpec₂ := by
-  --     have := transcript.rtake m (by omega)
-  --     sorry
-  --   let decision' ← V'.verify stmt secondTranscript
-  --   return decision ∧ decision'
+def OracleReduction.append (R₁ : OracleReduction pSpec₁ oSpec Stmt₁ Wit₁ Stmt₂ Wit₂)
+    (R₂ : OracleReduction pSpec₂ oSpec Stmt₂ Wit₂ Stmt₃ Wit₃) :
+      OracleReduction (pSpec₁ ++ₚ pSpec₂) oSpec Stmt₁ Wit₁ Stmt₃ Wit₃ where
+  prover := Prover.append R₁.prover R₂.prover
+  verifier := OracleVerifier.append R₁.verifier R₂.verifier
 
 -- Define composition of multiple protocols via recursion
 
 def ProtocolSpec.join (rounds : List ℕ)
     (pSpecs : ∀ i : Fin rounds.length, ProtocolSpec (rounds.get i)) :
     ProtocolSpec rounds.sum := sorry
-
-end Composition
-
-section Security
-
--- Show that composition preserves security properties such as completeness and (all variants of)
--- soundness.
-
-end Security
