ZKLib/OracleReduction.lean
@@ -1,3 +1,4 @@
 import ZKLib.OracleReduction.Basic
 import ZKLib.OracleReduction.Security
 import ZKLib.OracleReduction.Composition
+import ZKLib.OracleReduction.ToOracle
